Switch to new definitions and module system
* This includes lots of refactoring and new apis for things like
  iterators

Valaig/Aig/Basic.lean
@@ -1,210 +1,350 @@
-import Std.Sat.AIG.Basic
-import Std.Sat.AIG.CachedGates
-import Valaig.Aig.Defs
-import Valaig.Aig.DefsLemmas
-import Valaig.ForStd
+module
 
-open Valaig.Aig.Std
+public import Std.Sat.AIG.Basic
+public import Std.Sat.AIG.CachedGates
+public meta import Valaig.Prelude
+public import Valaig.Aig.StdSatLemmas
+public import Valaig.Aig.Refs
+public import Valaig.ForStd
 
-namespace Valaig.Aig.Raw
+namespace Valaig.Aig
 
-attribute [local simp, local grind] Raw.size
+/--
+The metadata of an input in the Aig.
+-/
+structure Input where
+  var : Var
 
-@[inline, simp]
-abbrev numInputs (aig : Raw) : Nat := aig.inputs.size
+namespace Input
+deriving instance Hashable, DecidableEq, Repr, Inhabited for Input
+end Input
 
-@[inline, simp]
-abbrev numLatches (aig : Raw) : Nat := aig.latches.size
+/--
+The metadata of a latch in the Aig.
+-/
+structure Latch where
+  var : Var
+  next : Lit
+  reset : Lit
 
--- Number of inputs and latches
-@[inline, simp, grind]
-def numAtoms (aig : Raw) : Nat := aig.numInputs + aig.numLatches
+namespace Latch
+deriving instance Hashable, DecidableEq, Repr, Inhabited for Latch
+end Latch
 
-@[inline]
-def maxVar (aig : Raw) : Var := .ofIdx (aig.size - 1)
+abbrev Inputs := Array Input
+abbrev Latches := Array Latch
 
-@[inline, simp]
-abbrev numConstants (_ : Raw) : Nat := 1
+end Valaig.Aig
 
--- Number of inputs, latches and constants
-@[inline, simp, grind]
-def numLeaves (aig : Raw) : Nat := aig.numAtoms + aig.numConstants
+-- Switch to public
+public section
+namespace Valaig.Aig
 
-@[inline, simp, grind]
-def numGates (aig : Raw) : Nat := aig.size - aig.numLeaves
+/--
+An index to an input definition in the Aig input array.
+-/
+structure InputIdx where
+  ofIdx ::
+    idx : Nat
 
-end Aig.Raw
+namespace InputIdx
+deriving instance DecidableEq, Repr, Inhabited, BEq, ReflBEq, LawfulBEq for InputIdx
+instance : Hashable InputIdx where hash := (hash ·.idx)
+instance : LawfulHashable InputIdx where hash_eq := by simp
+end InputIdx
 
-@[inline, simp]
-private abbrev Lit.In.ref {aig : Aig.Raw} (lit : Lit.In aig) : aig.aig.Ref :=
-  lit.val.toRef (by grind only [Var.validIn_def'])
+/--
+An index to a latch definition in the Aig latch array.
+-/
+structure LatchIdx where
+  ofIdx ::
+    idx : Nat
 
-namespace Aig
+namespace LatchIdx
+deriving instance DecidableEq, Repr, Inhabited, BEq, ReflBEq, LawfulBEq for LatchIdx
+instance : Hashable LatchIdx where hash := (hash ·.idx)
+instance : LawfulHashable LatchIdx where hash_eq := by simp
+end LatchIdx
 
-instance Raw.instGetElemVar : GetElem Raw Var (Std.Sat.AIG.Decl AtomIdx) (fun aig var => var.validIn aig) where
-  getElem aig var (h := by grind) := aig.aig.decls[var.idx]
+/--
+An atom in the combinational aig is either an input or a latch, which is just
+a reference back to the index in the inputs or latches arrays.
+-/
+inductive AtomIdx where
+| input (idx : InputIdx)
+| latch (idx : LatchIdx)
 
-@[inline, reducible, simp]
-instance instGetElemVar : GetElem Aig Var (Std.Sat.AIG.Decl AtomIdx) (fun aig var => var.validIn aig) where
-  getElem aig var (h := by grind) := aig.toRaw[var]'h
+namespace AtomIdx
+deriving instance Hashable, DecidableEq, Repr, Inhabited, BEq, ReflBEq, LawfulBEq for AtomIdx
+instance : LawfulHashable AtomIdx where hash_eq := by simp
+end AtomIdx
 
-instance Raw.instMem : Membership (Std.Sat.AIG.Decl AtomIdx) Raw where
-  mem aig decl := decl ∈ aig.aig.decls
+/--
+An output of interest in the circuit - this is also used to represent other
+nameable nodes in the Aiger format like bad and constraint nodes.
+-/
+structure Output where
+  lit : Lit
 
-@[inline, reducible, simp]
-instance instMem : Membership (Std.Sat.AIG.Decl AtomIdx) Aig where
-  mem aig decl := decl ∈ aig.toRaw
+namespace Output
+deriving instance Hashable, DecidableEq, Repr, Inhabited for Output
+end Output
 
-@[inline]
-def VarDef.idx (var : VarDef) (aig : Aig.Raw) (h : var.var.validIn aig := by grind)
-    (hatom : aig[var.var] matches .atom _ := by grind) : AtomIdx :=
-  match aig[var.var], hatom with
-  | .atom idx, _ => idx
-
-@[inline]
-def empty : Aig :=
-  {
-    aig := .empty
-    inputs := #[],
-    latches := #[],
-    hfalse := by simp [Std.Sat.AIG.empty],
-    hinputs := by simp [Std.Sat.AIG.empty],
-    hlatches := by simp [Std.Sat.AIG.empty],
-    hnexts := by simp,
-  }
-
-@[inline]
-def nextInputIdx (aig : Aig) : Nat :=
-  aig.numInputs
-
-@[inline]
-def nextLatchIdx (aig : Aig) : Nat :=
-  aig.numLatches
-
-@[inline]
-def addInput (aig : Aig) (symbol : String := "") : Aig × Input :=
-  -- We don't need to use mkAtomCached as nextInputIdx_notIn_decls guarantees
-  -- it would be a miss
-  let atom := (.input aig.nextInputIdx)
-  let res := aig.aig.mkAtom atom
-  let input := { var := .ofRef res.ref, symbol }
-
-  let aig := { aig with
-    aig := res.aig,
-    inputs := aig.inputs.push input,
-    hfalse := by apply hfalse_decls_push ?_ (by apply mkAtom_eq_decls_push) <;> grind only [hfalse],
-    hinputs := by
-      apply AtomsBij_push_push (by apply mkAtom_eq_decls_push) (by trivial) (hbijec := aig.hinputs)
-      · grind only [mkAtom_ref_eq_decls_size, Var.ofRef_idx]
-      · grind only [nextInputIdx]
-    hlatches := by apply AtomsBij_unchanged_push (by apply mkAtom_eq_decls_push) <;> grind only [hlatches],
-    hnexts := by grind only [validIn_push aig, mkAtom_eq_decls_push, hnexts]
-  }
-  (aig, input)
-
-@[inline]
-def addLatch (aig : Aig) (next : Lit) (reset : Lit) (symbol : String := "")
-    (hnext : next.validIn aig := by grind) (hreset : reset.validIn aig := by grind) : Aig × Latch :=
-  -- We don't need to use mkAtomCached as nextLatchIdx_notIn_decls guarantees
-  -- it would be a miss
-  let res := aig.aig.mkAtom <| .latch aig.nextLatchIdx
-  let latch := {
-    var := .ofRef res.ref,
-    next,
-    reset,
-    hreset := by simp_all [res, Var.validIn, Var.lt_idx, mkAtom_ref_eq_decls_size, Aig.Raw.size]
-    symbol
-  }
-
-  let aig := { aig with
-    aig := res.aig,
-    latches := aig.latches.push latch,
-    hfalse := by apply hfalse_decls_push ?_ (by apply mkAtom_eq_decls_push) <;> grind only [hfalse],
-    hinputs := by apply AtomsBij_unchanged_push (by apply mkAtom_eq_decls_push) <;> grind only [hinputs],
-    hlatches := by
-      apply AtomsBij_push_push (by apply mkAtom_eq_decls_push) (by trivial) (hbijec := aig.hlatches)
-      · grind only [mkAtom_ref_eq_decls_size, Var.ofRef_idx]
-      · grind only [nextLatchIdx]
-    hnexts := by grind only [validIn_push aig, mkAtom_eq_decls_push, Array.getElem_push, hnexts]
-  }
-  (aig, latch)
-
-@[inline]
-def addGate (aig : Aig) (rhs0 rhs1 : Lit)
-    (h0 : rhs0.validIn aig := by grind) (h1 : rhs1.validIn aig := by grind) :
-    Aig × Lit :=
-  let res := aig.aig.mkAndCached ⟨rhs0.toRef h0, rhs1.toRef h1⟩
-
-  let aig := { aig with
-    aig := res.aig,
-    hfalse := by
-      apply hfalse_decls_append aig.hfalse
-      · grind only [Std.Sat.AIG.mkAndCached_decl_eq]
-      · grind only [mkAndCached_matches_gate]
-      · apply Std.Sat.AIG.mkAndCached_le_size,
-    hinputs := by
-      apply AtomsBij_unchanged_append aig.hinputs
-      · apply Std.Sat.AIG.mkAndCached_le_size
-      · grind only [Std.Sat.AIG.mkAndCached_decl_eq]
-      · grind only [mkAndCached_matches_gate],
-    hlatches := by
-      apply AtomsBij_unchanged_append aig.hlatches
-      · apply Std.Sat.AIG.mkAndCached_le_size
-      · grind only [Std.Sat.AIG.mkAndCached_decl_eq]
-      · grind only [mkAndCached_matches_gate],
-    hnexts := by grind only [validIn_of_ge_size aig, Std.Sat.AIG.mkAndCached_le_size, hnexts, Aig.Raw.size]
-  }
-  (aig, Lit.ofRef res.ref)
-
-@[inline]
-def addGateUncached (aig : Aig) (rhs0 rhs1 : Lit)
-    (h0 : rhs0.validIn aig := by grind) (h1 : rhs1.validIn aig := by grind) :
-    Aig × Lit :=
-  let res := aig.aig.mkGate ⟨rhs0.toRef h0, rhs1.toRef h1⟩
-
-  let aig := { aig with
-    aig := res.aig,
-    hfalse := by
-      apply hfalse_decls_append aig.hfalse
-      · grind only [Std.Sat.AIG.mkGate_decl_eq]
-      · grind only [mkGate_matches_gate]
-      · apply Std.Sat.AIG.mkGate_le_size,
-    hinputs := by
-      apply AtomsBij_unchanged_append aig.hinputs
-      · apply Std.Sat.AIG.mkGate_le_size
-      · grind only [Std.Sat.AIG.mkGate_decl_eq]
-      · grind only [mkGate_matches_gate],
-    hlatches := by
-      apply AtomsBij_unchanged_append aig.hlatches
-      · apply Std.Sat.AIG.mkGate_le_size
-      · grind only [Std.Sat.AIG.mkGate_decl_eq]
-      · grind only [mkGate_matches_gate]
-    hnexts := by grind only [validIn_of_ge_size aig, Std.Sat.AIG.mkGate_le_size, hnexts, Aig.Raw.size]
-  }
-  (aig, Lit.ofRef res.ref)
-
-@[inline]
-def setNext (aig : Aig) (i : LatchIdx) (h : i < aig.numLatches)
-    (next : Lit) (hnext : next.validIn aig := by grind) : Aig :=
-  let latches := aig.latches.modifyMem i h ({ ·.val with next })
-  { aig with
-    latches,
-    hlatches := by constructor <;> grind [hlatches]
-    hnexts := by grind [hnexts, validIn_of_aig_eq aig]
-  }
-
-@[inline]
-def setNexts (aig : Aig) (f : (latch : Latch) -> latch ∈ aig.latches -> Lit.In aig) : Aig :=
-  let modify _ _ latch _ :=
-    let next := f latch (by grind only [Array.getElem_mem])
-    { latch with next }
-
-  { aig with
-    latches := aig.latches.mapMem modify
-    hlatches := by constructor <;> grind only [hlatches, Array.size_mapMem, Array.getElem_mapMem]
-    hnexts := by grind only [validIn_of_aig_eq aig, Array.getElem_mapMem]
-  }
+abbrev Outputs := Array Output
 
 end Aig
 
-end Valaig
+/--
+A sequential And-Inverter Graph consisting of inputs, latches and And gates. Outputs should be
+stored separately as `Lit`s in the `Aig`.
+-/
+structure Aig where
+  -- The underlying AIG
+  private aig : Std.Sat.AIG Aig.AtomIdx
+
+  -- A mapping from input indices (AtomIdx.input idx) to their definition
+  private inputs : Aig.Inputs
+
+  -- A mapping from latch indices (AtomIdx.latch idx) to their definition
+  private latches : Aig.Latches
+
+namespace Aig
+
+/--
+A representation of the node data stored for a particular variable in an `Aig`. For inputs and
+latches this requires a further lookup with `InputIdx.get` or `LatchIdx.get`.
+-/
+inductive Node where
+  | false
+  | input (idx : InputIdx)
+  | latch (idx : LatchIdx)
+  | and (lhs rhs : Lit)
+
+namespace Node
+deriving instance Hashable, DecidableEq, Repr, Inhabited for Node
+end Node
+
+/--
+An `Aig` with just the constant node.
+-/
+@[inline]
+def empty : Aig :=
+  {
+    aig := .empty,
+    inputs := #[],
+    latches := #[],
+  }
+
+/--
+The number of nodes currently allocated in aig.
+-/
+@[inline, local grind, local grind unfold]
+def size (aig : Aig) : Nat :=
+  aig.aig.decls.size
+
+/--
+The maximum variable currently allocated in the aig.
+-/
+@[inline]
+def maxVar (aig : Aig) : Var :=
+  .ofIdx <| aig.size - 1
+
+/--
+The number of input nodes in the aig.
+-/
+@[inline]
+def numInputs (aig : Aig) : Nat :=
+  aig.inputs.size
+
+/--
+The number of latch nodes in the aig.
+-/
+@[inline]
+def numLatches (aig : Aig) : Nat :=
+  aig.latches.size
+
+/--
+The number of gate nodes in the aig.
+-/
+@[inline, local simp, local grind unfold]
+abbrev numGates (aig : Aig) : Nat :=
+  aig.size - aig.numInputs - aig.numLatches - 1
+
+end Aig
+
+/-
+Variable accessors.
+-/
+
+namespace Var 
+
+def validIn (var : Var) (aig : Aig) : Prop :=
+  var.idx < aig.size
+
+@[inline]
+instance {var : Var} {aig : Aig} : Decidable (var.validIn aig) :=
+  have : var.validIn aig ↔ var.idx < aig.size := by
+    simp [Var.validIn]
+  decidable_of_iff' _ this
+
+end Var
+
+namespace Lit
+
+@[expose, reducible, simp, grind unfold]
+def validIn (lit : Lit) (aig : Aig) : Prop :=
+  lit.var.validIn aig
+
+@[inline]
+instance {lit : Lit} {aig : Aig} : Decidable (lit.validIn aig) :=
+  have : lit.validIn aig ↔ lit.var.validIn aig := by
+    simp [Lit.validIn]
+  decidable_of_iff' _ this
+
+end Lit
+
+@[always_inline]
+def Aig.get (aig : Aig) (var : Var) (valid : var.validIn aig := by grind) : Node :=
+  match aig.aig.decls[var.idx] with
+  | .false => .false
+  | .atom (.input idx) => .input idx
+  | .atom (.latch idx) => .latch idx
+  | .gate rhs0 rhs1 => .and (.ofFanin rhs0) (.ofFanin rhs1)
+
+@[inline, expose, reducible, simp, grind unfold]
+instance Aig.instGetElemVar : GetElem Aig Var Node (fun aig var => var.validIn aig) where
+  getElem aig var (h := by grind) :=
+    aig.get var h
+
+namespace Aig
+
+/-
+Input accessors.
+-/
+
+@[local simp]
+def InputIdx.validIn (idx : Aig.InputIdx) (aig : Aig) : Prop :=
+  idx.idx < aig.inputs.size
+deriving Decidable
+
+@[inline]
+def InputIdx.getVar (idx : Aig.InputIdx) (aig : Aig) (valid : idx.validIn aig := by grind) : Var :=
+  aig.inputs[idx.idx].var
+
+@[inline, simp]
+abbrev InputIdx.getLit (idx : Aig.InputIdx) (aig : Aig) (valid : idx.validIn aig := by grind) : Lit :=
+  idx.getVar aig valid |>.toLit
+
+/-
+Latch accessors.
+-/
+
+@[local simp]
+def LatchIdx.validIn (idx : Aig.LatchIdx) (aig : Aig) : Prop :=
+  idx.idx < aig.latches.size
+deriving Decidable
+
+@[inline]
+def LatchIdx.getVar (idx : Aig.LatchIdx) (aig : Aig) (valid : idx.validIn aig := by grind) : Var :=
+  aig.latches[idx.idx].var
+
+@[inline, simp]
+abbrev LatchIdx.getLit (idx : Aig.LatchIdx) (aig : Aig) (valid : idx.validIn aig := by grind) : Lit :=
+  idx.getVar aig valid |>.toLit
+
+@[inline]
+def LatchIdx.getNext (idx : Aig.LatchIdx) (aig : Aig) (valid : idx.validIn aig := by grind) : Lit :=
+  aig.latches[idx.idx].next
+
+@[inline]
+def LatchIdx.setNext (idx : Aig.LatchIdx) (aig : Aig) (next : Lit) (valid : idx.validIn aig := by grind) : Aig :=
+  { aig with latches := aig.latches.modifyMem idx.idx (by simp_all) ({ ·.val with next }) }
+
+@[inline]
+def LatchIdx.getReset (idx : Aig.LatchIdx) (aig : Aig) (valid : idx.validIn aig := by grind) : Lit :=
+  aig.latches[idx.idx].reset
+
+@[inline]
+def LatchIdx.setReset (idx : Aig.LatchIdx) (aig : Aig) (reset : Lit) (valid : idx.validIn aig := by grind) : Aig :=
+  { aig with latches := aig.latches.modifyMem idx.idx (by simp_all) ({ ·.val with reset }) }
+
+/--
+Arbitrary index validity and accessors, defined as abbreviations
+-/
+
+@[simp]
+abbrev AtomIdx.validIn (idx : Aig.AtomIdx) (aig : Aig) : Prop :=
+  match idx with
+  | .input idx => idx.validIn aig
+  | .latch idx => idx.validIn aig
+
+@[simp]
+abbrev AtomIdx.getVar (idx : Aig.AtomIdx) (aig : Aig) (valid : idx.validIn aig := by grind) : Var :=
+  match idx with
+  | .input idx => idx.getVar aig
+  | .latch idx => idx.getVar aig
+
+@[simp]
+abbrev AtomIdx.getLit (idx : Aig.AtomIdx) (aig : Aig) (valid : idx.validIn aig := by grind) : Lit :=
+  match idx with
+  | .input idx => idx.getLit aig
+  | .latch idx => idx.getLit aig
+
+instance : Coe InputIdx AtomIdx where
+  coe := (.input ·)
+
+instance : Coe LatchIdx AtomIdx where
+  coe := (.latch ·)
+
+/-
+Node constructors. There is no constant node constructor as the constant node always exists, so constant
+literals can be constructed with `Lit.true`/`Lit.false`.
+-/
+
+@[inline]
+def addInput (aig : Aig) : Aig × InputIdx :=
+  let idx := .ofIdx aig.inputs.size
+  let res := aig.aig.mkAtom <| .input idx
+  let input := { var := .ofRef res.ref }
+  let inputs := aig.inputs.push input
+  let aig := { aig with aig := res.aig, inputs }
+  (aig, idx)
+
+@[inline]
+def addLatch (aig : Aig) (next reset : Lit) : Aig × LatchIdx :=
+  let idx := .ofIdx aig.latches.size
+  let res := aig.aig.mkAtom <| .latch idx
+  let latch := { var := .ofRef res.ref, next, reset }
+  let latches := aig.latches.push latch
+  let aig := { aig with aig := res.aig, latches }
+  (aig, idx)
+
+-- TODO: Currently this requires proofs that rhs0/rhs1 are valid in the aig, but after switching to
+-- buffed (and getting rid of dependent typing) this won't be needed anymore
+@[inline]
+def addAnd (aig : Aig) (rhs0 rhs1 : Lit)
+    (valid0 : rhs0.validIn aig := by grind) (valid1 : rhs1.validIn aig := by grind) : Aig × Lit :=
+  let res := aig.aig.mkAndCached ⟨rhs0.toRef valid0, rhs1.toRef valid1⟩
+  let aig := { aig with aig := res.aig }
+  (aig, .ofRef res.ref)
+
+/-
+Setup get/set definitions for use locally as grind/simp rules, with grind_def/
+simp_def tactics to make use of them.
+-/
+attribute [simp_valaig_defs, grind_valaig_defs]
+  Aig.get Aig.instGetElemVar Aig.size
+  Aig.empty
+  InputIdx.getVar
+  LatchIdx.getVar LatchIdx.getNext LatchIdx.getReset
+  LatchIdx.setNext LatchIdx.setReset
+  Aig.addInput Aig.addLatch Aig.addAnd
+
+attribute [grind_valaig_defs] InputIdx LatchIdx
+attribute [grind_valaig_defs =_] Var.ext_idx
+
+attribute [simp_valaig_defs, grind_valaig_defs =]
+  Std.mkAtom_eq_decls_push Std.mkAtom_size Std.mkAtom_ref_eq_decls_size
+  Std.Sat.AIG.mkAndCached_decl_eq
+
+attribute [grind_valaig_defs! .] Std.Sat.AIG.mkAndCached_le_size
