Valaig/Aig/FromStd.lean
@@ -1,10 +1,18 @@
-import Valaig.Aig.Basic
-import Valaig.Aig.Lemmas
-import Std.Sat.AIG.Basic
-import Valaig.Prelude
+module
+
+public import Valaig.Prelude
+public import Valaig.Aig.Basic
+-- TODO: This shouldn't be necessary but the module system seems broken:
+-- https://github.com/leanprover/lean4/issues/12337
+import all Valaig.Aig.Basic
+public import Valaig.Aig.RefValidIn
+public import Valaig.Aig.GetSet
+public import Valaig.Aig.WellFormed
+public import Std.Sat.AIG.Basic
 
 -- Convert from a Std.Sat.AIG to our sequential Aig
 
+public section
 namespace Valaig.Aig
 
 open Std.Sat AIG
@@ -14,12 +22,7 @@ namespace FromStd
 
 inductive RelabelledAtom (aig : AIG α) where
 | input
-  (symbol : String := "")
-| latch
-  (next : aig.Ref)
-  -- TODO: Support generic reset functions and uninitialised latches not just Bool
-  (reset : Bool)
-  (symbol : String := "")
+| latch (next : aig.Ref) (reset : Bool)
 
 @[unbox, grind]
 private structure State (stdAig : AIG α) where
@@ -29,99 +32,98 @@ private structure State (stdAig : AIG α) where
   map : Array Lit := #[]
 
   -- A map from atoms in the original AIG to their canonical variable in aig
-  atomMap : Std.HashMap α Var := .emptyWithCapacity
+  atomMap : Std.HashMap α Aig.AtomIdx := .emptyWithCapacity
 
   -- A map from the variable defined by each latch to its ref in stdAig, to
   -- allow latch finalisation once all nodes have been visited
-  latchNexts : Std.HashMap Var stdAig.Ref := .emptyWithCapacity
+  latchNexts : Std.HashMap LatchIdx stdAig.Ref := .emptyWithCapacity
+
+  hwf : aig.WellFormed := by grind
 
   hmap : ∀ {x} (_ : x ∈ map), x.validIn aig := by grind
-  hlatch : ∀ {l} (_ : l ∈ aig.latches), l.var ∈ latchNexts := by grind
-  hatom : ∀ {a} (_ : a ∈ atomMap),
-    ∃ (h : atomMap[a].validIn aig), aig[atomMap[a]] matches .atom _ := by grind
+
+  hlatch : ∀ {l : LatchIdx} (_ : l.validIn aig), l ∈ latchNexts := by grind
+
+  hatom : ∀ {a} (_ : a ∈ atomMap), atomMap[a].validIn aig := by grind
 
 namespace State
 
 variable {aig : AIG α}
 
-@[simp, grind]
-abbrev size (s : State aig) := s.map.size
+@[always_inline, simp, grind]
+private abbrev size (s : State aig) := s.map.size
 
 @[simp, grind]
-def measure (s : State aig) := aig.decls.size - s.size
+private def measure (s : State aig) := aig.decls.size - s.size
 
-abbrev Pushed (s : State aig) := { s' : State aig // s'.size = s.size + 1 }
+private abbrev Pushed (s : State aig) := { s' : State aig // s'.size = s.size + 1 }
 
 @[always_inline]
-def addFalse (s : State aig) : s.Pushed :=
+private def addFalse (s : State aig) : s.Pushed :=
   ⟨{ s with map := s.map.push .false, hmap := by grind}, by grind only [Array.size_push]⟩
 
 @[always_inline]
-def addGate (s : State aig) (rhs0 rhs1 : Fanin)
+private def addGate (s : State aig) (rhs0 rhs1 : Fanin)
     (h0 : rhs0.gate < s.map.size) (h1 : rhs1.gate < s.map.size) : s.Pushed :=
   let rhs0 := s.map[rhs0.gate]'h0 |>.invert rhs0.invert
   let rhs1 := s.map[rhs1.gate]'h1 |>.invert rhs1.invert
-  rlet (aig, lhs) := s.aig.addGate rhs0 rhs1
+  rlet (aig, lhs) := s.aig.addAnd rhs0 rhs1
   let map := s.map.push lhs
 
-  have hmap := by grind only [addGate_validIn, validIn_addGate, Array.mem_push]
-  have hlatch := by grind only [addGate_latches_eq]
-  have hatom := by grind only [validIn_addGate, addGate_getElem_eq]
-  ⟨{ s with aig, map, hmap, hlatch, hatom }, by grind only [Array.size_push]⟩
+  have hmap := by grind
+  have hlatch := by grind
+  have hatom := by grind
+  have hwf := by grind
+  ⟨{ s with aig, map, hmap, hlatch, hatom, hwf }, by grind only [Array.size_push]⟩
 
 -- Tries to add an atom that already exists, returns none if it doesn't
 @[always_inline]
-def tryAddCachedAtom (s : State aig) (atom : α) : Option s.Pushed := do
-  rlet h : var ← s.atomMap[atom]?
-  let map := s.map.push var.toLit
+private def tryAddCachedAtom (s : State aig) (atom : α) : Option s.Pushed := do
+  rlet h : idx ← s.atomMap[atom]?
+  let map := s.map.push <| idx.getLit s.aig
 
   have hmap := by
-    simp_all
+    simp only [Array.mem_push]
     rintro _ (hold | hnew)
     · exact s.hmap hold
-    · have := Std.HashMap.isSome_getElem?_iff_mem.mp (Option.isSome_of_eq_some h)
-      simp_all; rw [←h]; cases (s.hatom this); trivial
+    · grind [@s.hwf.inputsValid, @s.hwf.latchesValid]
   return ⟨{ s with map, hmap }, by grind only [Array.size_push]⟩
 
 @[always_inline]
-def addInput (s : State aig) (atom : α) (symbol : String) : s.Pushed :=
-  let (eq:=_) (aig, input) := s.aig.addInput symbol
-  let map := s.map.push input
+private def addInput (s : State aig) (atom : α) : s.Pushed :=
+  let (eq:=_) (aig, input) := s.aig.addInput
+  let map := s.map.push <| input.getLit aig
   let atomMap := s.atomMap.insert atom input
 
-  have hmap := by simp; grind only [addInput_matches_atom, Lit.mk_eq_self, validIn_addInput, Lit.mk_ext]
-  have hlatch := by grind only [addInput_latches_eq]
-  have hatom := by
-    intros
-    simp only [Std.HashMap.getElem_insert]
-    split
-    · grind only [addInput_matches_atom]
-    · grind only [validIn_addInput, addInput_getElem_eq]
-  ⟨{ s with aig, map, atomMap, hmap, hlatch, hatom }, by grind only [Array.size_push]⟩
+  have hmap := by grind
+  have hlatch := by grind
+  have hatom := by grind
+  have hwf := by grind
+  ⟨{ s with aig, map, atomMap, hmap, hlatch, hatom, hwf }, by grind only [Array.size_push]⟩
 
 @[always_inline]
-def addLatch (s : State aig) (atom : α) (next : aig.Ref) (reset : Bool) (symbol : String) : s.Pushed :=
+private def addLatch (s : State aig) (atom : α) (next : aig.Ref) (reset : Bool) : s.Pushed :=
   let nextLit := Lit.ofRef next
   let resetLit := Lit.constant reset
 
   -- We set a fake next state literal at first because we may not have added the logic driving
   -- the next state yet and store it in latchNexts so we can update it subsequently
-  let (eq:=_) (aig, latch) := s.aig.addLatch .false resetLit symbol
-  let map := s.map.push latch
+  let (eq:=_) (aig, latch) := s.aig.addLatch .false resetLit
+  let map := s.map.push <| latch.getLit aig
   let atomMap := s.atomMap.insert atom latch
   let latchNexts := s.latchNexts.insert latch next
 
-  have hmap := by simp; grind only [addLatch_matches_atom, Lit.mk_eq_self, validIn_addLatch, Lit.mk_ext]
-  have hlatch := by simp; grind only [addLatch_latches_eq_push, Array.mem_push]
-  have hatom := by simp; grind only [addLatch_matches_atom, validIn_addLatch, Std.HashMap.getElem_insert, addLatch_getElem_eq]
-  ⟨{ aig, map, atomMap, latchNexts, hmap, hlatch, hatom }, by grind only [Array.size_push]⟩
+  have hlatch := by grind
+  have hatom := by grind
+  have hwf := by grind
+  ⟨{ aig, map, atomMap, latchNexts, hmap := by grind, hlatch, hatom, hwf }, by grind⟩
 
 end State
 
 structure Result (stdAig : AIG α) where
   aig : Aig
   refMap : stdAig.Ref -> Lit
-  atomMap : α -> Option Var
+  atomMap : α -> Option AtomIdx
 
   hrefvalid : ∀ {ref}, refMap ref |>.validIn aig
 
@@ -131,23 +133,11 @@ open FromStd in
 def fromStdAIG (stdAig : AIG α) (relabel : α -> RelabelledAtom stdAig) : Result stdAig :=
   have ⟨state, hstate⟩ := go
 
-  let aig := state.aig.setNexts <| fun latch h =>
-    let ref := state.latchNexts[latch.var]'(state.hlatch h)
-    have := ref.hgate
-    let lit := state.map[ref.gate]'(by omega) |>.invert ref.invert
-    ⟨lit, by grind [!Lit.mk_var]⟩
-
   let refMap (ref : stdAig.Ref) : Lit :=
     have := ref.hgate
     state.map[ref.gate]'(by omega) |>.invert ref.invert
 
-  let atomMap (atom : α) : Option Var := state.atomMap[atom]?
-
-  have hrefvalid : ∀ {ref}, refMap ref |>.validIn aig := by
-    simp [refMap]
-    grind only [validIn_setNexts, Array.getElem_mem]
-
-  { aig, refMap, atomMap, hrefvalid }
+  { aig := state.aig, refMap, atomMap := (state.atomMap[·]?), hrefvalid := by grind }
 
 where
   go (s : State stdAig := {}) (h : s.map.size ≤ stdAig.decls.size := by grind) :
@@ -167,20 +157,11 @@ where
           | some s => s
           | none =>
             match relabel atom with
-            | .input            symbol => s.addInput atom symbol
-            | .latch next reset symbol => s.addLatch atom next reset symbol
+            | .input            => s.addInput atom
+            | .latch next reset => s.addLatch atom next reset
 
       have : s'.measure < s.measure := by grind only [State.measure]
       go s' (by lia)
   termination_by s.measure
-
-/-
-@[inline]
-def fromStdEntrypoint (entry : Entrypoint α) (relabel : α -> RelabelledAtom entry.aig) :
-    (result : FromStdResult entry.aig) × (Lit.In result.aig) :=
-  let result := fromStdAIG entry.aig relabel
-  let lit := result.refMap entry.ref
-  ⟨result, ⟨lit, result.hrefvalid⟩⟩
--/
 
 end Valaig.Aig
