Valaig/Aig/Iter.lean
@@ -1,0 +1,169 @@
+module
+
+public import Valaig.Aig.Basic
+import all Valaig.Aig.Basic
+public import Valaig.Aig.RefValidIn
+
+public section
+namespace Valaig.Aig
+
+/-
+Iterator types for iterating over valid indices/variables in the Aig.
+-/
+
+/--
+A generic iterator that forward iterates over a range of valid indices. This
+is specialised to produce input/latch indices and variables.
+-/
+structure GenericIter {α : Type} (mk : Nat -> α) (size : Nat) (valid : α -> Prop) where
+  idx : Nat
+
+namespace GenericIter
+
+class LawfulValid {α : Type} (mk : Nat -> α) (size : Nat) (valid : α -> Prop) : Prop where
+  hvalid : ∀ {out : α}, valid out ↔ ∃ (n : Nat) (_ : out = mk n), n < size
+
+universe u
+variable {α : Type} {mk : Nat -> α} {size : Nat} {valid : α -> Prop}
+variable {m : Type -> Type u} [Pure m]
+
+@[inline]
+instance instIterator : Std.Iterator (GenericIter mk size valid) m α where
+  IsPlausibleStep it step :=
+    match step with
+    | .yield it' out =>
+      it.internalState.idx < size ∧
+      it'.internalState.idx = it.internalState.idx + 1 ∧
+      out = mk it.internalState.idx
+    | .skip _ => False
+    | .done => 
+      it.internalState.idx ≥ size
+
+  step it := pure <| .deflate <|
+    let s := it.internalState
+    if h : s.idx < size then
+      .yield ⟨⟨s.idx + 1⟩⟩ (mk s.idx) (by grind)
+    else
+      .done (by grind)
+
+attribute [local grind =] Std.IterM.Step.toPure_yield
+attribute [local grind =] Std.IterM.Step.toPure_skip
+attribute [local grind =] Std.IterM.Step.toPure_done
+attribute [local grind unfold] Std.PlausibleIterStep.yield
+attribute [local grind unfold] Std.PlausibleIterStep.skip
+attribute [local grind unfold] Std.PlausibleIterStep.done
+attribute [local grind =] Std.IterStep.successor_yield
+attribute [local grind =] Std.IterStep.successor_skip
+attribute [local grind =] Std.IterStep.successor_done
+attribute [local simp, local grind unfold] Std.Iterator.step Std.Iter.step Std.IterM.step
+attribute [local simp, local grind unfold] Std.Iter.toIterM Std.IterM.toIter
+attribute [local grind =] Std.Shrink.inflate_deflate
+attribute [local grind .] Std.Iter.IsPlausibleIndirectOutput.direct
+attribute [local grind .] Std.Iter.IsPlausibleIndirectOutput.indirect
+attribute [local simp, local grind unfold] Std.IterM.IsPlausibleSuccessorOf
+attribute [local simp, local grind unfold] Std.IterM.IsPlausibleStep
+attribute [local simp, local grind unfold] Std.Iter.IsPlausibleStep
+attribute [local simp, local grind unfold] Std.Iterator.IsPlausibleStep
+attribute [local simp] Std.Iter.IsPlausibleOutput
+attribute [local simp] Std.Iter.IsPlausibleSuccessorOf
+attribute [local simp, local grind unfold] Std.IterM.IsPlausibleSuccessorOf
+attribute [local simp, local grind unfold] Std.IterM.IsPlausibleOutput
+attribute [local grind =] Std.IterStep.mapIterator_yield
+
+open Std.Iterators in
+private def instFinitenessRelation : FinitenessRelation (GenericIter mk size valid) m where
+  Rel := InvImage WellFoundedRelation.rel (size - ·.internalState.idx)
+  wf := InvImage.wf _ WellFoundedRelation.wf
+  subrelation {it it'} h := by simp_wf; grind
+
+instance instFinite [Pure m] : Std.Iterators.Finite (GenericIter mk size valid) m := by
+  exact .of_finitenessRelation instFinitenessRelation
+
+@[always_inline]
+instance instIteratorLoop [Monad m] [Monad n] :
+    Std.IteratorLoop (GenericIter mk size valid) m n :=
+  .defaultImplementation
+
+variable {it : @Std.Iter (GenericIter mk size valid) α} {out : α}
+
+@[simp, grind =]
+theorem IsPlausibleOutput_iff :
+    it.IsPlausibleOutput out ↔
+      it.internalState.idx < size ∧ out = mk it.internalState.idx := by
+  simp
+  intros
+  exists ⟨⟨it.internalState.idx + 1⟩⟩
+
+@[simp, grind =]
+theorem IsPlausibleSuccessorOf_iff {it' : @Std.Iter (GenericIter mk size valid) α} :
+    it'.IsPlausibleSuccessorOf it ↔
+      it.internalState.idx < size ∧
+      it'.internalState.idx = it.internalState.idx + 1 := by
+  constructor
+  · grind [Std.Iter.IsPlausibleSuccessorOf]
+  · rw [Std.Iter.isPlausibleSuccessorOf_iff_exists]
+    intro h
+    exists .yield ⟨⟨it.internalState.idx + 1⟩⟩ (mk it.internalState.idx)
+    constructor
+    · simp
+      congr
+      grind
+    · grind
+
+@[simp, grind =]
+theorem IsPlausibleIndirectOutput_iff :
+    it.IsPlausibleIndirectOutput out ↔
+      ∃ (n : Nat) (_ : n < size) (_ : n ≥ it.internalState.idx), mk n = out := by
+  constructor
+  · intro h
+    induction h <;> grind
+  · rintro ⟨n, h1, h2, h3⟩
+    induction h : (size - it.internalState.idx) generalizing it
+    case zero => grind
+    case succ n' ih =>
+      by_cases n = it.internalState.idx
+      · grind
+      · let it' := it.step.val.successor.get <| by grind
+        apply Std.Iter.IsPlausibleIndirectOutput.indirect (it' := it')
+        · grind
+        · apply ih <;> grind
+
+@[simp, grind =]
+theorem IsPlausibleIndirectOutput_toIterM_iff :
+    it.toIterM.IsPlausibleIndirectOutput out ↔
+      ∃ (n : Nat) (_ : n < size) (_ : n ≥ it.internalState.idx), mk n = out := by
+  rw [←Std.Iter.isPlausibleIndirectOutput_iff_isPlausibleIndirectOutput_toIterM]
+  simp
+
+@[always_inline, inline]
+instance instForIn' [Monad n] [lawful : LawfulValid mk size valid] :
+    ForIn' n (@Std.Iter (GenericIter mk size valid) α) α ⟨fun _ out => valid out⟩ where
+  forIn' it init f :=
+    Std.IteratorLoop.finiteForIn' (fun _ _ f c => f c.run) |>.forIn' it.toIterM init
+      fun out h acc => f out (by grind [lawful.hvalid]) acc
+
+end GenericIter
+
+abbrev InputIterator (aig : Aig) := GenericIter InputIdx.ofIdx aig.numInputs (·.validIn aig)
+instance {aig : Aig} : GenericIter.LawfulValid InputIdx.ofIdx aig.numInputs (·.validIn aig) where
+  hvalid := by grind [InputIdx.validIn, numInputs]
+
+@[inline]
+def inputIter (aig : Aig) : @Std.Iter (InputIterator aig) InputIdx :=
+  ⟨⟨0⟩⟩
+
+abbrev LatchIterator (aig : Aig) := GenericIter LatchIdx.ofIdx aig.numLatches (·.validIn aig)
+instance {aig : Aig} : GenericIter.LawfulValid LatchIdx.ofIdx aig.numLatches (·.validIn aig) where
+  hvalid := by grind [LatchIdx.validIn, numLatches]
+
+@[inline]
+def latchIter (aig : Aig) : @Std.Iter (LatchIterator aig) LatchIdx :=
+  ⟨⟨0⟩⟩
+
+abbrev VarIterator (aig : Aig) := GenericIter Var.ofIdx aig.size (·.validIn aig)
+instance {aig : Aig} : GenericIter.LawfulValid Var.ofIdx aig.size (·.validIn aig) where
+  hvalid := by grind [Var.validIn]
+
+@[inline]
+def iter (aig : Aig) : @Std.Iter (VarIterator aig) Var :=
+  ⟨⟨0⟩⟩
