Valaig/Aiger.lean
@@ -1,3 +1,5 @@
-import Valaig.Aiger.Basic
-import Valaig.Aiger.Parser
-import Valaig.Aiger.Writer
+module
+
+public import Valaig.Aiger.Basic
+public import Valaig.Aiger.Parser
+public import Valaig.Aiger.Writer
