Valaig/Aiger/Writer.lean
@@ -1,5 +1,10 @@
-import Valaig.Aiger.Basic
+module
 
+public import Valaig.Aiger.Basic
+import all Valaig.Aig.Basic
+public import Valaig.Aig.Iter
+
+public section
 namespace Valaig.Aiger
 
 def writeAag (aiger : Aiger) (file : IO.FS.Stream) : IO Unit := do
@@ -8,23 +13,21 @@ def writeAag (aiger : Aiger) (file : IO.FS.Stream) : IO Unit := do
   file.putStrLn s!"aag {aig.maxVar.idx} {aig.numInputs} {aig.numLatches} 0 {aig.numGates} {aiger.numBads} 0 0 0"
 
   -- Input lines
-  for input in aig.inputs do
-    file.putStrLn s!"{input.var.toLit.idx}"
+  for h : input in aig.inputIter do
+    file.putStrLn s!"{input.getLit aig |>.idx}"
 
   -- Latch lines
-  for h : latch in aig.latches do
-    file.putStrLn s!"{latch.lit.idx} {latch.next.idx} {latch.reset.idx}"
+  for h : latch in aig.latchIter do
+    file.putStrLn s!"{latch.getLit aig |>.idx} {latch.getNext aig |>.idx} {latch.getReset aig |>.idx}"
 
   -- Bad lines
   for bad in aiger.bads do
     file.putStrLn s!"{bad.lit.idx}"
 
   -- Gates
-  for h : i in [0:aig.size] do
-    if let .gate rhs0 rhs1 := aig.aig.decls[i] then
-      let (rhs0, rhs1) := (Lit.ofFanin rhs0, Lit.ofFanin rhs1)
-      let lhs := Var.ofIdx i |>.toLit
-      file.putStrLn s!"{lhs.idx} {rhs0.idx} {rhs1.idx}"
+  for h : var in aig.iter do
+    if let .and rhs0 rhs1 := aig[var] then
+      file.putStrLn s!"{var.toLit.idx} {rhs0.idx} {rhs1.idx}"
 
   -- TODO: Symbols/comments
   file.flush
